#Theorem [[Homomorphisms]]
Let $f$ be a homomorphism from $G$ to $G$'.Denote by K the set of all elements of $G$ which are mapped to the identity element of $G^\prime$,$i. e.$ $K= \{ a\in G;$ $a\xrightarrow{\mathbf{f}}e^{\prime}\in G^{\prime}\}.$ Then K forms an [[Invariant Subgroup]] of $G.$ Furthermore, the factor $\operatorname{group}G/K$ is isomorphic to $G^\prime.$

$\begin{array}{ll}{\mathsf{Proof:}}&{(\mathrm{i)~If~}a,b\in\mathcal{K},\mathrm{~then~}ab\xrightarrow{\mathrm{f}}e^{\prime}\cdot e^{\prime}=e^{\prime}.\mathrm{~Hence~}ab\in\mathcal{K}.\mathrm{~For~a~homomor-}}\\{\mathsf{phism,~we~must~have~}e\in G\xrightarrow{\mathrm{f}}e^{\prime}\in G^{\prime}\mathrm{~and~}g^{-1}\xrightarrow{\mathrm{f}}g^{\prime-1}(\mathrm{if~}g\xrightarrow{\mathrm{f}}g^{\prime}).\mathrm{~Hence}}\end{array}$ $e\in K$,and if $a\in K$ then $a^-1\xrightarrow{\mathrm{f}}(e^{\prime})^{-1}=e^{\prime}$ which implies that $a^-1\in K.$ Therefore K is a subgroup.
(ii) Let$a\in K$ and $g$ be any element of $G.$ We have: $gag^-1\xrightarrow{\mathrm{f}}g^{\prime}e^{\prime}(g^{-1})^{\prime}=g^{\prime}e^{\prime}g^{\prime-1}$ $=e^{\prime}.$ Hence $gag^-1\in K$ for all $g\in G.$ This means that K is an invariant subgroup. (iii) The elements of the factor group $G/K$ are cosets $pK.$ Consider the mapping $pK\xrightarrow{\rho }p^{\prime }\in G^{\prime }$ (where $p\xrightarrow{\mathrm{f} }p^{\prime }) .$ If $\rho ( pK) = \rho ( qK)$, then $\rho ( q^{- 1}p\tilde{K} )$ $= \rho ( q^{- 1}K\cdot pK) = \rho ( q^{- 1}K) \rho ( pK) = \rho ^{- 1}( qK) \rho ( pK) = e^{\prime }$ which implies that $q^{- 1}pK= K$ or $qK= pK$,Thus the mapping is one- to- one. Group multiplication is preserved by $\rho$, as $\rho(pK)\rho(qK)=p^{\prime}q^{\prime}=(p\tilde{q})^{\prime}=\rho(pqK).$ Therefore, $\rho$ is an isomorphism. K is often called the kernel or center of the homomorphism $f.$ We show schematically the content of this theorem in Fig.2.5a and Fig.2.5b. $QED$